\section*{Task 6.2}

\subsection*{Task statement}

Solve system $\begin{cases}
    y_1^{\prime} = 6y_1 - y_2 \\
    y_2^{\prime} = y_1 + 4y_2
\end{cases}$

\subsection*{Solution}

Let us differentiate the first equation:

\[y_1^{\prime \prime} = 6y_1^{\prime} - y_2^{\prime}\]

After instantiating the second equation into it, we obtain:

\[y_1^{\prime \prime} = 6y_1^{\prime} - y_1 - 4y_2\]

From the first equation: $y_2 = 6y_1 - y_1^{\prime}$. Let us instantiate it in the equation above:

\[y_1^{\prime \prime} = 10y_1^{\prime} - 25y_1\]

The equation obtained is a linear homogeneous second order differential equation.

\begin{displaymath}
    \begin{aligned}
        y_1^{\prime \prime} - 10y_1^{\prime} + 25y_1 & = 0 \\ 
        a^2 e^{ax} - 10a e^{ax} + 25 e^{ax} & = 0 \\
        a^2 - 10a + 25 & = 0 \\
        a & = 5
    \end{aligned}
\end{displaymath}

Hence $y_1 = C_1 e^{5x} + C_2 x e^{5x}$.

We know that $y_2 = 6y_1 - y_1^{\prime}$, hence $y_2 = C_1 e^{5x} + C_2 x e^{5x} - C_2 e^{5x}$

\subsection*{Answer}

The solution for given system is: $\begin{pmatrix}
y_1 \\ y_2
\end{pmatrix} = C_1 \begin{pmatrix}
    e^{5x} \\ e^{5x}
\end{pmatrix} + C_2 \begin{pmatrix}
    x e^{5x} \\ -e^{5x} + x e^{5x}
\end{pmatrix}$