\section*{Task 6.3}

\subsection*{Task statement}

Solve system $\begin{cases}
    y_1^{\prime} = 5y_1 + 2y_2 \\
    y_2^{\prime} = -4y_1 + y_2
\end{cases}$

\subsection*{Solution}

Let us differentiate the first equation:

\[y_1^{\prime \prime} = 5y_1^{\prime} + 2y_2^{\prime}\]

After instantiating the second equation into it, we obtain:

\[y_1^{\prime \prime} = 5y_1^{\prime} - 8y_1 + 2y_2\]

From the first equation: $y_2 = \frac{y_1^{\prime} - 5y_1}{2}$. Let us instantiate it in the equation above:

\[y_1^{\prime \prime} = 6y_1^{\prime} - 13y_1\]

The equation obtained is a linear homogeneous second order differential equation.

\begin{displaymath}
    \begin{aligned}
        y_1^{\prime \prime} - 6y_1^{\prime} + 13y_1 & = 0 \\ 
        a^2 e^{ax} - 6a e^{ax} + 13 e^{ax} & = 0 \\
        a^2 - 6a + 13 & = 0 \\
        a & = 3 \pm 2i
    \end{aligned}
\end{displaymath}

Hence 
\begin{displaymath}
    \begin{aligned}
        y_1 & = C_1 e^{(3 + 2i)x} + C_2 e^{(3 - 2i)x} \\
        & = C_1 e^{3x} e^{2ix} + C_2 e^{3x} e^{-2ix} \\
        & = e^{3x} (C_1 \cos{2x} + C_1 i \sin{2x} + C_2 \cos{2x} - C_2 i \sin{2x}) \\
        & = e^{3x} ((C_1 + C_2) \cos{2x} + i(C_1 - C_2) \sin{2x}) \\
        & = e^{3x} (D_1 \cos{2x} + D_2 \sin{2x})
    \end{aligned}
\end{displaymath}

We know that $y_2 = \frac{y_1^{\prime} - 5y_1}{2}$, hence $y_2 = \frac{e^{3x}}{2} (3(D_1 \cos{2x} + D_2 \sin{2x}) + 2(D_2 \cos{2x} - D_1 \sin{2x}) - 5(D_1 \cos{2x} + D_2 \sin{2x})) = -D_1 e^{3x} (\cos{2x} + \sin{2x}) + D_2(\cos{2x} - \sin{2x})$

\subsection*{Answer}

The solution for given system is: $\begin{pmatrix}
y_1 \\ y_2
\end{pmatrix} = - D_1 e^{3x} \begin{pmatrix}
    \cos{2x} \\ \cos{2x} + \sin{2x}
\end{pmatrix} + D_2 e^{3x} \begin{pmatrix}
    \sin{2x} \\ \cos{2x} - \sin{2x}
\end{pmatrix}$