\section*{Task 6.5}

\subsection*{Task statement}

Solve system $y_1^{\prime} = 2y_1 + 3y_2$ and $y_2^{\prime} = 4y_1 - 2y_2$ using matrix exponent, eigenvalues and eigenvectors.

\subsection*{Solution}

Representation of the system in matrix form:

\[\begin{pmatrix} y_1 \\ y_2 \end{pmatrix} = e^{\begin{pmatrix} 2 & 3 \\ 4 & -2 \end{pmatrix}x} \begin{pmatrix} C_1 \\ C_2 \end{pmatrix} \]

To find matrix exponential, we need to find eigenvalues and eigenvectors:

\begin{itemize}
    \item Eigenvalues:
    \begin{displaymath}
        \begin{aligned}
            det \begin{pmatrix} 2 - \lambda & 3 \\ 4 & -2 - \lambda \end{pmatrix} & = 0 \\
            (2 - \lambda)(-2 - \lambda) - 12 & = 0 \\
            \lambda^2 - 4 - 12 & = 0 \\
            \lambda & = \pm 4
        \end{aligned}
    \end{displaymath}
    \item Eigenvectors:
        \begin{enumerate}
            \item $\lambda = 4$:
                \begin{displaymath}
                    \begin{aligned}
                        \begin{pmatrix} -2 & 3 \\ 4 & -6 \end{pmatrix} \begin{pmatrix} x_1 \\ x_2 \end{pmatrix} & = 0 \\
                        \begin{pmatrix} x_1 \\ x_2 \end{pmatrix} & = \begin{pmatrix} 3 \\ 2 \end{pmatrix} \\
                        v_1 & = \begin{pmatrix} 3 \\ 2 \end{pmatrix}
                    \end{aligned}
                \end{displaymath}
            \item $\lambda = -4$:
                \begin{displaymath}
                    \begin{aligned}
                        \begin{pmatrix} 6 & 3 \\ 4 & 2 \end{pmatrix} \begin{pmatrix} x_1 \\ x_2 \end{pmatrix} & = 0 \\
                        \begin{pmatrix} x_1 \\ x_2 \end{pmatrix} & = \begin{pmatrix} -1 \\ 2 \end{pmatrix} \\
                        v_2 & = \begin{pmatrix} -1 \\ 2 \end{pmatrix}
                    \end{aligned}
                \end{displaymath}
        \end{enumerate}
    \item Matrix exponential:
        
        Let $V = \begin{pmatrix} v_1 & v_2 \end{pmatrix} = \begin{pmatrix} 3 & -1 \\ 2 & 2 \end{pmatrix}$

        \begin{displaymath}
            \begin{aligned}
                e^{\begin{pmatrix} 2 & 3 \\ 4 & -2 \end{pmatrix}x} & = V e^{\Lambda x} V^{-1} \\
                & = \begin{pmatrix} 3 & -1 \\ 2 & 2 \end{pmatrix} e^{\begin{pmatrix} 4 & 0 \\ 0 & -4 \end{pmatrix}} \frac{1}{4} \begin{pmatrix} -1 & \frac{3}{2} \\ 1 & \frac{1}{2} \end{pmatrix} \\
                & = \frac{1}{4} \begin{pmatrix} e^{-4x} + 3e^{4x} & \frac{3}{2} (e^{4x} - e^{-4x}) \\ 2(e^{4x} - e^{-4x}) & 3e^{-4x} + e^{4x} \end{pmatrix}
            \end{aligned}
        \end{displaymath}
\end{itemize}

Hence the solution is $\begin{pmatrix} y_1 \\ y_2 \end{pmatrix} = \frac{1}{4} \begin{pmatrix} e^{-4x} + 3e^{4x} & \frac{3}{2} (e^{4x} - e^{-4x}) \\ 2(e^{4x} - e^{-4x}) & 3e^{-4x} + e^{4x} \end{pmatrix} \begin{pmatrix} C_1 \\ C_2 \end{pmatrix}$.

Or:

\begin{displaymath}
    \begin{aligned}
        y_1 & = C_1(e^{-4x} + 3e^{4x}) + C_2(e^{4x} - e^{-4x}) \\
        y_2 & = C_1(e^{4x} - e^{-4x}) + C_2(3e^{-4x} + e^{4x})
    \end{aligned}
\end{displaymath}

\subsection*{Answer}

The solution for the system: 
\begin{displaymath}
    \begin{aligned}
        y_1 & = C_1(e^{-4x} + 3e^{4x}) + C_2(e^{4x} - e^{-4x}) = D_1e^{-4x} + D_2e^{4x} \\
        y_2 & = C_1(e^{4x} - e^{-4x}) + C_2(3e^{-4x} + e^{4x}) = D_3e^{-4x} + D_4e^{4x}
    \end{aligned}
\end{displaymath}