\section*{Task 7.2}

\subsection*{Task statement}

If $n \in \mathbf{N}$ then $L(t^n e^{at}) = $ if $s > a$ then $\frac{n!}{(s - a)^{n + 1}}$ else undefined.

\subsection*{Solution}

\begin{displaymath}
    \begin{aligned}
        L(t^n e^{at}) & = \int_0^{\infty} t^n e^{(a - s)t} dt \\
        & = \frac{t^n e^{(a - s)t}}{a - s} \Bigr|_0^{\infty} - \int_0^{\infty} nt^{n - 1} \frac{e^{(a - s)t}}{a - s} dt \\
        & = \frac{n}{s - a} \int_0^{\infty} t^{n - 1} e^{(a - s)t}
    \end{aligned}
\end{displaymath}

Hence $L(t^n e^{at}) = \frac{n}{s - a} L(e^{at} t^{n - 1})$

\begin{itemize}
    \item For $n = 1$:
    
        $L(t^1 e^{at}) = \frac{1}{s - a} L(e^{at} t^0) = \frac{1}{(s - a)^2}$ (According to the first shift property)
    
    \item For $n = 2$:
    
        $L(t^2 e^{at}) = \frac{2}{s - a} L(e^{at} t^1) = \frac{2}{(s - a)^3}$

    \item For $n = 3$:
    
        $L(t^3 e^{at}) = \frac{3}{s - a} L(e^{at} t^2) = \frac{6}{(s - a)^4}$
\end{itemize}

Hence $L(t^n e^{at}) = \frac{n!}{(s - a)^{n + 1}}$ for $s > a$.
