\section*{Task 5.14}

\subsection*{Task statement}

Show that the equation $y'' - 6y' - 9y = 0$ has a general solution $y = (C_1 + C_2 x)e^{3x}$. What is the most general solution of this
equation?

\subsection*{Solution}

The equation is a linear homogeneous second order ordinary differential equation.

Let $y = e^{ax}$, then

\[a^2 e^{ax} - 6a e^{ax} + 9 e^{ax} = 0\]
\[a^2 - 6a - 9 = 0\]

Solving this equation, we obtain the root $a = 3$.

We have a mulitple root, hence we should adopt $y_1 = e^{3x}$ as the first partial solution of the equation.

To do it, I will use variable variation to find an independent particular solution $y_2 = zy_1 = ze^{3x}$.

The derivatives of $y_2$:

\begin{displaymath}
    \begin{aligned}
        y_2^{\prime} & = z' e^{3x} + 3z e^{3x} \\
        y_2^{\prime \prime} & = z'' e^{3x} + 3z' e^{3x} + 3z' e^{3x} + 9z e^{3x} = e^{3x}(z'' + 6z' + 9z)
    \end{aligned}
\end{displaymath}

Instantiating $y_2,\ y_2^{\prime} \ y_2^{\prime \prime}$ in to the equation we obtain:

\begin{displaymath}
    \begin{aligned}
        e^{3x}(z'' + 6z' + 9z) - 6e^{3x} (z' + 3z) + 9ze^{3x} & = 0 \\
        z'' + 6z' + 9z - 6z' - 18z + 9z & = 0 \\
        z'' & = 0 
    \end{aligned}
\end{displaymath}

Integrating $z''$ by $x$ we obtain:

\begin{displaymath}
    \begin{aligned}
        z' & = \int 0 dx = C_2 \\
        z & = \int C_2 dx = C_2 x + C_1
    \end{aligned}
\end{displaymath}

Hence we obtain the solution: $y_2 = (C_1 + C_2x)e^{3x}$. It contains of two partial solutions: $C_1 e^{3x}$ and $C_2x e^{3x}$. They are linearly independent, therefore the solution is the most general.

\subsection*{Answer}

The solution $y = (C_1 + C_2x)e^{3x}$ is a general solution (shown above) and it is the most general.
